Add conc DSL, doc updates, and Shao ignore rules

examples/ConcChan.v
@@ -12,25 +12,67 @@ Section ConcChan.
   Let P := {| conc_val := Val; conc_tid := Tid; conc_chan := Chan |}.
 
   Variable ThreadState SharedState : Type.
+  Definition merge_shared (l r : SharedState) : SharedState := r.
+  Variable default_tid : Tid.
+  Variable delivered : Val.
+  Variable ch : Chan.
+  Variable payload : Val.
 
   Notation config := (ConcStrategy.config ThreadState SharedState).
   Notation term := (ConcMonad.conc_term P).
+  Import ConcMonad.Notations.
+  Local Open Scope conc_scope.
 
-  Definition sender (ts : ThreadState) : term ThreadState := ConcMonad.ret ts.
-  Definition receiver (ts : ThreadState) : term ThreadState := ConcMonad.ret ts.
+  Definition chan_handlers : ConcStrategy.handlers P ThreadState SharedState :=
+    {|
+      ConcStrategy.h_spawn := fun sh => ((default_tid : conc_tid P), sh, None);
+      ConcStrategy.h_yield := fun sh => sh;
+      ConcStrategy.h_send  := fun _ _ sh => sh;
+      ConcStrategy.h_recv  := fun _ sh => (delivered, sh);
+      ConcStrategy.h_join  := fun _ sh => (delivered, sh);
+    |}.
+
+  Definition pick_head (c : config) : option nat :=
+    match ConcStrategy.cfg_threads ThreadState SharedState c with
+    | [] => None
+    | _ => Some 0
+    end.
+
+  (** Thread program: send a payload, then receive on the same channel, keeping the state. *)
+  Definition send_then_recv (ts : ThreadState) : term ThreadState :=
+    _ <- ConcMonad.send (P:=P) ch payload (fun _ => ConcMonad.ret tt);;
+    _ <- ConcMonad.recv (P:=P) ch (fun _ => ConcMonad.ret ts);;
+    ConcMonad.ret ts.
 
   Definition compose_config (t1 t2 : ThreadState) (sh : SharedState) : config :=
     {| ConcStrategy.cfg_threads := [t1; t2];
        ConcStrategy.cfg_shared := sh |}.
 
-  Definition R : term config -> config -> Prop := fun t c => ConcRefinement.R_conc P ThreadState SharedState t c.
+  Definition R : term config -> config -> Prop :=
+    ConcRefinement.R_conc P ThreadState SharedState
+                          chan_handlers pick_head send_then_recv.
 
-  (** Placeholder correctness statement. *)
+  (** The specification that returns its input configuration refines itself. *)
   Lemma chan_example_refines :
     forall t1 t2 sh, R (ConcMonad.ret (compose_config t1 t2 sh)) (compose_config t1 t2 sh).
   Proof.
     intros t1 t2 sh.
     unfold R.
     apply ConcRefinement.ret_refines.
+  Qed.
+
+  (** A concrete scheduler step executes the send/recv program without changing the state. *)
+  Lemma chan_step_progress :
+    forall sh tstate,
+      ConcStrategy.step P ThreadState SharedState
+        chan_handlers pick_head send_then_recv
+        {| ConcStrategy.cfg_threads := [tstate]; ConcStrategy.cfg_shared := sh |}
+        {| ConcStrategy.cfg_threads := [tstate]; ConcStrategy.cfg_shared := sh |}.
+  Proof.
+    intros sh tstate.
+    refine (@ConcStrategy.step_run P ThreadState SharedState
+              chan_handlers pick_head send_then_recv
+              {| ConcStrategy.cfg_threads := [tstate]; ConcStrategy.cfg_shared := sh |}
+              0 tstate tstate sh [] _ _ _); simpl; auto.
   Qed.
 End ConcChan.
